src/util/list/sort.lean
@@ -233,11 +233,7 @@ begin
   exact xs_ih h,
 end
 
-theorem sorted_ne_eq {t: Type} {xs ys: list t}
-  [has_le t]
-  [has_lt t]:
-  (∀ (x y: t), x ≤ y -> x ≠ y -> x < y) ->
-  (∀ (x y: t), ¬ (x < y ∧ y < x)) ->
+theorem sorted_ne_eq {t: Type} {xs ys: list t} [decidable_linear_order t]:
   (∀ (x: t), x ∈ xs ↔ x ∈ ys) ->
   pairwise ne xs ->
   pairwise ne ys ->
@@ -245,7 +241,7 @@ theorem sorted_ne_eq {t: Type} {xs ys: list t}
   sorted ys ->
   xs = ys :=
 begin
-  intros lt_of_le_ne not_lt_both x_in p_xs p_ys s_xs s_ys,
+  intros x_in p_xs p_ys s_xs s_ys,
   induction xs generalizing ys,
   exact symm (iff.elim_left nothing_mem_nil (fun x xi,
     list.not_mem_nil x (iff.elim_right (x_in x) xi))),
@@ -281,10 +277,6 @@ begin
   exact p_ys_a xs_hd h h_1,
   let a := s_ys_a xs_hd h,
   let b := s_xs_a ys_hd h_1,
-  let c := p_ys_a xs_hd h,
-  let c' := fun h, c (symm h),
-  let a' := lt_of_le_ne ys_hd xs_hd a c,
-  let b' := lt_of_le_ne xs_hd ys_hd b c',
   exfalso,
-  exact not_lt_both ys_hd xs_hd (and.intro a' b'),
+  exact p_ys_a xs_hd h (le_antisymm a b),
 end
